intermediate/Veritas.Intermediate.VerifyS.fsti
@@ -127,8 +127,7 @@ let vaddm (s:slot_id) (r:record) (s':slot_id) (vs: vtls {Valid? vs}): vtls =
               (* check hashes match and k was not evicted to blum *)
               if not (h2 = h && b2 = false) then Failed
               (* check store does not contain k*)
-              else if Left? d && l_child_in_store st s' then Failed
-              else if Right? d && r_child_in_store st s' then Failed
+              else if child_in_store st s' d then Failed
               else 
                 let st_upd = add_to_store st s k v Spec.MAdd in
                 let st_upd2 = update_in_store st_upd s' d true in
@@ -161,6 +160,18 @@ let has_instore_merkle_desc (st:vstore) (s:slot_id{store_contains st s}): bool =
     Desc? ld && l_child_in_store st s || 
     Desc? rd && r_child_in_store st s
 
+let update_hash_and_blum_bit 
+      (st:vstore) 
+      (s:slot_id{store_contains st s /\ MVal? (stored_value st s)}) 
+      (d:bin_tree_dir{Desc? (desc_hash_dir (to_merkle_value (stored_value st s)) d)}) 
+      (h:hash_value)
+      (b:bool)
+  : vstore
+  = let mv = to_merkle_value (stored_value st s) in
+    let Desc k _ _ = desc_hash_dir mv d in
+    let mv' = Spec.update_merkle_value mv d k h b in
+    update_value st s (MVal mv')
+
 let vevictm (s:slot_id) (s':slot_id) (vs: vtls {Valid? vs}): vtls = 
   let st = thread_store vs in
   (* check store contains s and s' *)
@@ -186,8 +197,7 @@ let vevictm (s:slot_id) (s':slot_id) (vs: vtls {Valid? vs}): vtls =
       | Desc k2 h2 b2 -> 
           if k2 <> k then Failed
           else
-            let v'_upd = Spec.update_merkle_value v' d k h false in
-            let st_upd = update_value st s' (MVal v'_upd) in
+            let st_upd = update_hash_and_blum_bit st s' d h false in
             let st_upd2 = evict_from_store st_upd s in
             update_thread_store vs st_upd2
 
@@ -265,15 +275,10 @@ let vevictbm (s:slot_id) (s':slot_id) (t:timestamp) (vs:vtls {Valid? vs}): vtls 
       | Desc k2 h2 b2 -> 
           if k2 <> k || b2 then Failed
           else
-            let v'_upd = Spec.update_merkle_value v' d k h2 true in
-            let st_upd = update_value st s' (MVal v'_upd) in
+            let st_upd = update_hash_and_blum_bit st s' d h2 true in
             vevictb s t (update_thread_store vs st_upd)
 
 (* Relation between SC and S thread-local states *)
-
-let hashes_diverged (hadd:ms_hash_value) (hevict:ms_hash_value) : bool = 
-  // TODO: informally, there is no way to extend the add or evict sets so that their hashes match
-  admit()
   
 let vtls_rel (vs:vtls) (vs':SC.vtls) : Type =
   (Failed? vs /\ SC.Failed? vs') \/
@@ -282,12 +287,8 @@ let vtls_rel (vs:vtls) (vs':SC.vtls) : Type =
     let (SC.Valid id' st' clk' ha' he') = vs' in
     // all fields are equal
     equal_contents st st' /\ id = id' /\ clk = clk' /\ ha = ha' /\ he = he' /\
-    // SC's is_map field indicates that the add/evict sets have diverged -- not needed?
-    (not (SC.thread_store_is_map vs') ==> hashes_diverged ha he) /\
-    // the invariant over MAdd keys always holds
-    merkle_store_inv st /\ 
-    // the invariant over BAdd keys holds if the add/evict sets have not diverged
-    (not (hashes_diverged ha he) ==> blum_store_inv st)))
+    // the invariant over MAdd keys holds
+    merkle_store_inv st))
 
 let lemma_vget_simulates_SC 
       (vs:vtls{Valid? vs})
@@ -297,19 +298,12 @@ let lemma_vget_simulates_SC
       (v:data_value)
   : Lemma (requires (vtls_rel vs vs'))
           (ensures (vtls_rel (vget s k v vs) (SC.vget s k v vs')))
-          // TODO: add a condition to each 'ensures' that says that the add/evict hashes stay diverged
   = ()
 
 let lemma_update_value_DVal_preserves_merkle_inv (st:vstore) (s:slot_id{store_contains st s /\ is_data_key (stored_key st s)}) (v:data_value)
   : Lemma (requires merkle_store_inv st)
           (ensures merkle_store_inv (update_value st s (DVal v)))
           [SMTPat (merkle_store_inv (update_value st s (DVal v)))]
-  = admit()
-
-let lemma_update_value_DVal_preserves_blum_inv (st:vstore) (s:slot_id{store_contains st s /\ is_data_key (stored_key st s)}) (v:data_value)
-  : Lemma (requires blum_store_inv st)
-          (ensures blum_store_inv (update_value st s (DVal v)))
-          [SMTPat (blum_store_inv (update_value st s (DVal v)))]
   = admit()
 
 let lemma_vput_simulates_SC
@@ -338,7 +332,7 @@ let lemma_vaddm_simulates_SC
       then
         let k' = stored_key st s' in
         let v' = stored_value st s' in
-        if is_proper_desc k k' && not (store_contains st s) && not (DVal? v')
+        if is_proper_desc k k' && not (store_contains st s) && is_value_of k v && not (DVal? v')
         then
           let v' = to_merkle_value v' in
           let d = desc_dir k k' in
@@ -349,34 +343,34 @@ let lemma_vaddm_simulates_SC
           | Empty -> 
               // CASE 1 - by points_to_nearest_desc_in_store, either k is not in the store or 
               //          the final hash check is guaranteed to fail
-              assert (points_to_nearest_desc_in_store st s' Spec.MAdd);
-              // ==> not (store_contains_key_with_am st k Spec.MAdd)
+              assert (points_to_nearest_desc_in_store st s');
               if v = init_value k 
               then (
                 let v'_upd = Spec.update_merkle_value v' d k h false in
                 let st_upd = update_value st s' (MVal v'_upd) in
                 let st_upd2 = add_to_store st_upd s k v Spec.MAdd in
                 let st_upd3 = update_in_store st_upd2 s' d true in
-                assume (merkle_store_inv st_upd3);
-                if (not (hashes_diverged (thread_hadd vs) (thread_hevict vs)))
-                then (
-                  assert (points_to_nearest_desc_in_store st s' Spec.BAdd);
-                  // ==> not (store_contains_key_with_am st k Spec.BAdd)
-                  assume (blum_store_inv st_upd3) // easy(?) since we're not adding anything via BAdd
-                )
+                assume (merkle_store_inv st_upd3)
               )
           | Desc k2 h2 b2 -> 
               if k2 = k 
               // CASE 2 - by in_store_flag_implies.. and evicted_to_blum_flag_implies.., either 
               //          k is not in the store or the final hash check is guaranteed to fail
               then (
-                assert (in_store_flag_unset_implies_desc_not_in_store st s');              
+                assert (in_store_flag_unset_equals_desc_not_in_store st s');              
                 if h2 = h && b2 = false
-                then admit() // TODO...
+                then 
+                if not (child_in_store st s' d)
+                then (
+                  assert (not (store_contains_key_with_MAdd st k));
+                  let st_upd = add_to_store st s k v Spec.MAdd in
+                  let st_upd2 = update_in_store st_upd s' d true in
+                  assume (merkle_store_inv st_upd2)
+                )
               )
               // CASE 3 - similar to CASE 1
               else (
-                assert (points_to_nearest_desc_in_store st s' Spec.MAdd);              
+                assert (points_to_nearest_desc_in_store st s');              
                 if v = init_value k && is_proper_desc k2 k 
                 then
                   let d2 = desc_dir k2 k in
@@ -387,26 +381,14 @@ let lemma_vaddm_simulates_SC
                   let st_upd2 = add_to_store st_upd s k (MVal mv_upd) Spec.MAdd in
                   let st_upd3 = update_in_store st_upd2 s' d true in
                   let st_upd4 = update_in_store st_upd3 s d2 true in
-                  assume (merkle_store_inv st_upd4);                  
-                  assert (SC.Valid? (SC.vaddm s r s' vs'));
-                  if (not (hashes_diverged (thread_hadd vs) (thread_hevict vs)))
-                  then (
-                    assert (points_to_nearest_desc_in_store st s' Spec.BAdd);
-                    assume (blum_store_inv st_upd4)
-                  )
+                  assume (merkle_store_inv st_upd4)
               )
 #pop-options
 
-let lemma_evict_from_store_preserves_merkle_inv (st:vstore) (s:slot_id{store_contains st s})
+let lemma_evict_from_store_preserves_inv (st:vstore) (s:slot_id{store_contains st s})
   : Lemma (requires merkle_store_inv st)
           (ensures merkle_store_inv (evict_from_store st s))
           [SMTPat (merkle_store_inv (evict_from_store st s))]
-  = admit()
-
-let lemma_update_evict_from_store_preserves_blum_inv (st:vstore) (s:slot_id{store_contains st s})
-  : Lemma (requires blum_store_inv st)
-          (ensures blum_store_inv (evict_from_store st s))
-          [SMTPat (blum_store_inv (evict_from_store st s))]
   = admit()
 
 let lemma_has_in_store_merkle_desc (st:vstore) (st':SCstore.vstore) (s:slot_id{store_contains st s})
@@ -415,39 +397,30 @@ let lemma_has_in_store_merkle_desc (st:vstore) (st':SCstore.vstore) (s:slot_id{s
           [SMTPat (has_instore_merkle_desc st s); SMTPat (SC.has_instore_merkle_desc st' (SCstore.stored_key st' s))]
   = admit()
 
+let lemma_update_hash_and_blum_bit_preserves_inv 
+      (st:vstore) 
+      (s:slot_id{store_contains st s /\ MVal? (stored_value st s)}) 
+      (d:bin_tree_dir{Desc? (desc_hash_dir (to_merkle_value (stored_value st s)) d)}) 
+      (h:hash_value)
+      (b:bool)
+  : Lemma (requires merkle_store_inv st)
+          (ensures merkle_store_inv (update_hash_and_blum_bit st s d h b)) 
+          [SMTPat (merkle_store_inv (update_hash_and_blum_bit st s d h b))]
+  = admit()
+
 let lemma_vevictm_simulates_SC 
       (vs:vtls{Valid? vs}) 
       (vs':SC.vtls{SC.Valid? vs'}) 
       (s s':slot_id)  
   : Lemma (requires (vtls_rel vs vs'))
           (ensures (vtls_rel (vevictm s s' vs) (SC.vevictm s s' vs'))) 
-  = let st = thread_store vs in
-    let st' = SC.thread_store vs' in
-    if store_contains st s && store_contains st s'
-    then 
-      let k = stored_key st s in
-      let v = stored_value st s in
-      let k' = stored_key st s' in
-      let v' = stored_value st s' in
-      if is_proper_desc k k' && not (has_instore_merkle_desc st s) 
-      then
-        let d = desc_dir k k' in
-        let _ = assert (is_value_of k' v') in 
-        let v' = to_merkle_value v' in
-        let dh' = desc_hash_dir v' d in
-        let h = hashfn v in
-        match dh' with
-        | Empty -> ()
-        | Desc k2 h2 b2 ->
-            if k2 = k
-            then
-              let v'_upd = Spec.update_merkle_value v' d k h false in
-              let st_upd = update_value st s' (MVal v'_upd) in
-              let st_upd2 = evict_from_store st_upd s in
-              let Valid id st clk ha he = update_thread_store vs st_upd2 in
-              assume (merkle_store_inv st_upd);
-              if not (hashes_diverged ha he) 
-              then assume (blum_store_inv st_upd)
+  = ()
+
+let lemma_add_to_store_BAdd_preserves_inv (st:vstore) (s:st_index st{not (store_contains st s)}) (k:key) (v:value_type_of k)
+  : Lemma (requires merkle_store_inv st)
+          (ensures merkle_store_inv (add_to_store st s k v Spec.BAdd))
+          [SMTPat (merkle_store_inv (add_to_store st s k v Spec.BAdd))]
+  = admit()
 
 let lemma_vaddb_simulates_SC 
       (vs:vtls{Valid? vs}) 
@@ -458,46 +431,7 @@ let lemma_vaddb_simulates_SC
       (j:thread_id)
   : Lemma (requires (vtls_rel vs vs'))
           (ensures (vtls_rel (vaddb s r t j vs) (SC.vaddb s r t j vs')))
-  = if s < thread_store_size vs
-    then
-      let st = thread_store vs in 
-      let (k,v) = r in
-      if is_value_of k v
-      then if not (store_contains st s)
-      then
-        let h = thread_hadd vs in
-        let h_upd = ms_hashfn_upd (MHDom (k,v) t j) h in
-        let vs_upd = update_thread_hadd vs h_upd in
-        let clk = thread_clock vs in
-        let clk_upd = Spec.max clk (next t) in
-        let vs_upd2 = update_thread_clock vs_upd clk_upd in
-        let st_upd = add_to_store st s k v Spec.BAdd in
-        let Valid _ st _ ha he = update_thread_store vs_upd2 st_upd in
-        assume (merkle_store_inv st); // easy since we are not adding anything via MAdd
-        assume (not (SC.thread_store_is_map (SC.vaddb s r t j vs')) ==> hashes_diverged ha he);  
-        assume (not (hashes_diverged ha he) ==> blum_store_inv st)
-
-(* Thoughts on filling in the last two assumes:
-
-   if store_contains_key k
-   then (
-     the SC is_map flag will be false
-     hashes_diverged should be true
-     -> blum_store_inv st does not need to hold
-   )
-   else (
-     SC will leave the is_map flag unchanged
-     if blum_store_inv is violated by adding k
-     then (
-       there exists a slot s s.t.
-       (a) k is marked as a descendent of s and the evicted_to_blum flag of s is not set 
-       or (b) k is a descendent of s, but is not stored in the hash of s
-
-       ... in either case, the hashes have diverged
-     )
-     -> this proves (not hashes_diverged ==> blum_store_inv holds)
-   )
-*)
+  = ()
 
 let lemma_vevictb_simulates_SC 
       (vs:vtls{Valid? vs}) 
@@ -506,21 +440,8 @@ let lemma_vevictb_simulates_SC
       (t:timestamp)
   : Lemma (requires (vtls_rel vs vs'))
           (ensures (vtls_rel (vevictb s t vs) (SC.vevictb s t vs'))) 
-  = let clock = thread_clock vs in
-    let st = thread_store vs in
-    if store_contains st s 
-    then
-      let k = stored_key st s in
-      let v = stored_value st s in
-      if k <> Root && ts_lt clock t && add_method_of st s = Spec.BAdd && not (has_instore_merkle_desc st s)
-      then
-        let h = thread_hevict vs in
-        let h_upd = ms_hashfn_upd (MHDom (k,v) t (thread_id_of vs)) h in
-        let vs_upd = update_thread_hevict vs h_upd in
-        let vs_upd2 = update_thread_clock vs_upd t in    
-        let st_upd = evict_from_store st s in
-        let Valid _ _ _ ha he = update_thread_store vs_upd2 st_upd in
-        if (hashes_diverged ha he) then assume (blum_store_inv st)
+          [SMTPat (vtls_rel (vevictb s t vs) (SC.vevictb s t vs'))]
+  = ()
 
 let lemma_vevictbm_simulates_SC 
       (vs:vtls{Valid? vs}) 
@@ -529,34 +450,8 @@ let lemma_vevictbm_simulates_SC
       (t:timestamp)
   : Lemma (requires (vtls_rel vs vs'))
           (ensures (vtls_rel (vevictbm s s' t vs) (SC.vevictbm s s' t vs'))) 
-  = let st = thread_store vs in
-    if store_contains st s && store_contains st s' 
-    then
-      let k = stored_key st s in
-      let k' = stored_key st s' in
-      let v' = stored_value st s' in
-      if is_proper_desc k k' && add_method_of st s = Spec.MAdd && not (has_instore_merkle_desc st s)
-      then
-        let _ = assert (is_value_of k' v') in 
-        let v' = to_merkle_value v' in
-        let d = desc_dir k k' in
-        let dh' = desc_hash_dir v' d in
-        match dh' with
-        | Empty -> ()
-        | Desc k2 h2 b2 -> 
-            if k2 = k && not b2 
-            then (
-              let v'_upd = Spec.update_merkle_value v' d k h2 true in
-              let st_upd = update_value st s' (MVal v'_upd) in
-              let st' = SC.thread_store vs' in
-              let st_upd' = SCstore.update_store st' s' (MVal v'_upd) in
-              let Valid id st clk ha he = update_thread_store vs st_upd in
-              assume (merkle_store_inv st_upd); // same assumes as vevictm
-              if not (hashes_diverged ha he) 
-              then assume (blum_store_inv st_upd);
-              lemma_vevictb_simulates_SC (update_thread_store vs st_upd) (SC.update_thread_store vs' st_upd') s t
-            )
-
+  = ()
+  
 let t_verify_step (vs:vtls) (e:logS_entry): vtls =
   match vs with
   | Failed -> Failed
@@ -570,7 +465,7 @@ let t_verify_step (vs:vtls) (e:logS_entry): vtls =
     | EvictB_S s t -> vevictb s t vs
     | EvictBM_S s s' t -> vevictbm s s' t vs
 
-(* Verify a log from a specified initial state *)
+(* Verify a (thread-local) log from a specified initial state *)
 let rec t_verify_aux (vs:vtls) (l:logS): Tot vtls
   (decreases (Seq.length l)) =
   let n = Seq.length l in
@@ -581,4 +476,63 @@ let rec t_verify_aux (vs:vtls) (l:logS): Tot vtls
     let e = Seq.index l (n - 1) in
     t_verify_step vsp e
 
-// ... 
+(* Initialize verifier state *)
+// TODO: what should the initial size be?
+let store_size = 65536 // 2 ^ 16
+let init_thread_state (id:thread_id): vtls = 
+  let vs = Valid id (empty_store store_size) (MkTimestamp 0 0) empty_hash_value empty_hash_value in  
+  if id = 0 then
+    let st0 = thread_store vs in
+    let st0_upd = add_to_store st0 0 Root (init_value Root) Spec.MAdd in
+    update_thread_store vs st0_upd    
+  else vs
+
+(* Main thread-level verify function *)
+let t_verify (id:thread_id) (l:logS): vtls = 
+  t_verify_aux (init_thread_state id) l 
+
+val init_thread_state_valid (id:thread_id)
+  : Lemma (Valid? (init_thread_state id))
+          [SMTPat (init_thread_state id)]
+
+val lemma_init_thread_state_rel (id:thread_id)
+  : Lemma (vtls_rel (init_thread_state id) (SC.init_thread_state id))
+
+val lemma_t_verify_simulates_SC (id:thread_id) (l:logS) 
+  : Lemma (vtls_rel (t_verify id l) (SC.t_verify id l))
+
+(* Global verification *)
+let verify (tl:thread_id_logS): vtls =
+  t_verify (fst tl) (snd tl)
+  
+let verifiable (gl: g_logS) = 
+  forall (tid:seq_index gl). Valid? (verify (thread_log gl tid))
+
+let verifiable_log = gl:g_logS{verifiable gl}
+
+val hadd (gl: verifiable_log): ms_hash_value
+
+val hevict (gl: verifiable_log): ms_hash_value
+
+let hash_verifiable (gl: verifiable_log): bool = 
+  hadd gl = hevict gl
+
+let hash_verifiable_log = gl:verifiable_log{hash_verifiable gl}
+
+let lemma_verifiable_simulates_SC (gl:verifiable_log)
+  : Lemma (ensures SC.verifiable gl)
+          [SMTPat (SC.verifiable gl)]
+  = admit()
+
+let lemma_hash_verifiable_simulates_SC (gl:hash_verifiable_log)
+  : Lemma (SC.hash_verifiable gl)
+  = admit() 
+    // requires showing that hash check succeeds ==> SC returns is_map=true for every thread
+    // alternatively, if SC returns is_map=false for any thread, then the hash check will fail
+
+(* Correctness *)
+
+let lemma_verifier_correct (gl: hash_verifiable_log { ~ (Veritas.State.seq_consistent (to_state_op_glogS gl))})
+  : Veritas.Verifier.EAC.hash_collision_gen
+  = lemma_hash_verifiable_simulates_SC gl;
+    SC.lemma_verifier_correct gl
